cedar-lean/Cedar/Thm/Validation/Levels/And.lean
@@ -35,12 +35,11 @@ open Cedar.Spec
 open Cedar.Validation
 
 theorem level_based_slicing_is_sound_and {e₁ e₂ : Expr} {n : Nat} {c₀ c₁: Capabilities} {env : Environment} {request : Request} {entities slice : Entities}
-  (hn : nmax ≥ n)
-  (hs : slice = entities.sliceAtLevel request nmax)
+  (hs : slice = entities.sliceAtLevel request n)
   (hc : CapabilitiesInvariant c₀ request entities)
   (hr : RequestAndEntitiesMatchEnvironment env request entities)
   (ht : typeOf (.and e₁ e₂) c₀ env = Except.ok (tx, c₁))
-  (hl : TypedExpr.AtLevel tx n nmax)
+  (hl : TypedExpr.AtLevel tx n)
   (ih₁ : TypedAtLevelIsSound e₁)
   (ih₂ : TypedAtLevelIsSound e₂)
   : evaluate (.and e₁ e₂) request entities = evaluate (.and e₁ e₂) request slice
@@ -55,7 +54,7 @@ theorem level_based_slicing_is_sound_and {e₁ e₂ : Expr} {n : Nat} {c₀ c₁
     replace hv₁ := instance_of_ff_is_false hv₁
     subst v₁
     cases hl ; rename_i hl₁
-    specialize ih₁ hn hs hc hr htx₁ (by assumption)
+    specialize ih₁ hs hc hr htx₁ (by assumption)
     simp only [evaluate, ←ih₁]
     rcases he₁ with he₁ | he₁ | he₁ | he₁ <;>
     simp [he₁, Result.as, Coe.coe, Value.asBool]
@@ -64,11 +63,11 @@ theorem level_based_slicing_is_sound_and {e₁ e₂ : Expr} {n : Nat} {c₀ c₁
     replace ⟨ b₁ , hv₁⟩ := instance_of_bool_is_bool hv₁
     subst v₁ tx
     cases hl ; rename_i hl₁ hl₂
-    specialize ih₁ hn hs hc hr htx₁ hl₁
+    specialize ih₁ hs hc hr htx₁ hl₁
     simp only [evaluate, ←ih₁]
     rcases he₁ with he₁ | he₁ | he₁ | he₁ <;>
     simp only [he₁, Result.as, Bool.not_eq_eq_eq_not, Bool.not_true, Coe.coe, Value.asBool, Except.bind_err]
     cases b₁ <;> simp only [Except.bind_ok, ↓reduceIte]
     specialize hgc he₁
-    specialize ih₂ hn hs (capability_union_invariant hc hgc) hr htx₂ hl₂
+    specialize ih₂ hs (capability_union_invariant hc hgc) hr htx₂ hl₂
     simp [ih₂]
