cedar-lean/Cedar/Thm/Validation/Levels/BinaryApp.lean
@@ -47,32 +47,27 @@ theorem not_dereferencing_apply₂_invariant_entities {op : BinaryOp} {entities 
     ) <;>
     simp
 
-theorem level_based_slicing_is_sound_inₑ {e₁ : Expr} {euid₁ euid₂ : EntityUID} {n nmax : Nat} {c₀ c₁ : Capabilities} {entities slice : Entities}
-  (hn : nmax ≥ n + 1)
+theorem level_based_slicing_is_sound_inₑ {e₁ : Expr} {euid₁ euid₂ : EntityUID} {n : Nat} {c₀ c₁ : Capabilities} {entities slice : Entities}
   (hc : CapabilitiesInvariant c₀ request entities)
   (hr : RequestAndEntitiesMatchEnvironment env request entities)
   (ht : typeOf e₁ c₀ env = Except.ok (tx₁, c₁))
-  (hl : TypedExpr.AtLevel tx₁ n nmax)
+  (hl : TypedExpr.EntityAccessAtLevel tx₁ n (n + 1))
   (hel : ¬ TypedExpr.EntityLitViaPath tx₁ [])
   (he : evaluate e₁ request entities = .ok (Value.prim (Prim.entityUID euid₁)))
-  (hs : some slice = entities.sliceAtLevel request nmax)
+  (hs : some slice = entities.sliceAtLevel request (n + 1))
   : inₑ euid₁ euid₂ entities = inₑ euid₁ euid₂ slice
 := by
   simp only [inₑ]
   cases heq : euid₁ == euid₂ <;> simp only [Bool.false_or, Bool.true_or]
-  replace hl : TypedExpr.AtLevel tx₁ (nmax - 1) nmax :=
-    check_level_greater (by omega) hl
-  rw [(by simp at hn ; omega : nmax = nmax - 1 + 1)] at hs
   have hfeq := checked_eval_entity_find_entities_eq_find_slice hc hr ht hl hel he hs
   simp [hfeq, Entities.ancestorsOrEmpty]
 
 theorem level_based_slicing_is_sound_binary_app {op : BinaryOp} {e₁ e₂ : Expr} {n : Nat} {c₀ c₁: Capabilities} {env : Environment} {request : Request} {entities slice : Entities}
-  (hn : nmax ≥ n)
-  (hs : slice = entities.sliceAtLevel request nmax)
+  (hs : slice = entities.sliceAtLevel request n)
   (hc : CapabilitiesInvariant c₀ request entities)
   (hr : RequestAndEntitiesMatchEnvironment env request entities)
   (ht : typeOf (.binaryApp op e₁ e₂) c₀ env = Except.ok (tx, c₁))
-  (hl : TypedExpr.AtLevel tx n nmax)
+  (hl : TypedExpr.AtLevel tx n)
   (ihe₁ : TypedAtLevelIsSound e₁)
   (ihe₂ : TypedAtLevelIsSound e₂)
   : evaluate (.binaryApp op e₁ e₂) request entities = evaluate (.binaryApp op e₁ e₂) request slice
@@ -82,10 +77,10 @@ theorem level_based_slicing_is_sound_binary_app {op : BinaryOp} {e₁ e₂ : Exp
   simp only [evaluate]
   cases hl
   case getTag hel hl₁ hl₂ | hasTag hel hl₁ hl₂ =>
-    specialize ihe₂ (by omega) hs hc hr htx₂ hl₂
+    specialize ihe₂ hs hc hr htx₂ hl₂
     rw [←ihe₂]
-    have hl₁' := check_level_succ hl₁
-    specialize ihe₁ hn hs hc hr htx₁ hl₁'
+    have hl₁' := entity_access_at_level_then_at_level (by omega) hl₁
+    specialize ihe₁ hs hc hr htx₁ hl₁'
     rw [←ihe₁]
     cases he₁ : evaluate e₁ request entities <;> simp only [Except.bind_ok, Except.bind_err]
     cases he₂ : evaluate e₂ request entities <;> simp only [Except.bind_ok, Except.bind_err]
@@ -94,16 +89,13 @@ theorem level_based_slicing_is_sound_binary_app {op : BinaryOp} {e₁ e₂ : Exp
     rename_i p₁ p₂
     cases p₁ <;> cases p₂ <;> simp only
     rename_i euid _
-    replace hl₁ : TypedExpr.AtLevel tx₁ (nmax - 1) nmax :=
-      check_level_greater (by omega) hl₁
-    rw [(by simp at hn ; omega : nmax = nmax - 1 + 1)] at hs
     have hfeq := checked_eval_entity_find_entities_eq_find_slice hc hr htx₁ hl₁ hel he₁ hs
     simp only [hfeq, hasTag, getTag, Entities.tagsOrEmpty, Entities.tags, Map.findOrErr]
   case mem hel hl₁ hl₂ =>
-    specialize ihe₂ (by omega) hs hc hr htx₂ hl₂
+    specialize ihe₂ hs hc hr htx₂ hl₂
     rw [←ihe₂]
-    have hl₁' := check_level_succ hl₁
-    specialize ihe₁ hn hs hc hr htx₁ hl₁'
+    have hl₁' := entity_access_at_level_then_at_level (by omega) hl₁
+    specialize ihe₁ hs hc hr htx₁ hl₁'
     rw [←ihe₁]
     cases he₁ : evaluate e₁ request entities <;> simp only [Except.bind_ok, Except.bind_err]
     cases he₂ : evaluate e₂ request entities <;> simp only [Except.bind_ok, Except.bind_err]
@@ -112,13 +104,13 @@ theorem level_based_slicing_is_sound_binary_app {op : BinaryOp} {e₁ e₂ : Exp
     case prim =>
       rename_i p₁ p₂
       cases p₁ <;> cases p₂ <;> simp only
-      simp [level_based_slicing_is_sound_inₑ hn hc hr htx₁ hl₁ hel he₁ hs]
+      simp [level_based_slicing_is_sound_inₑ hc hr htx₁ hl₁ hel he₁ hs]
     case set =>
       rename_i p₁ sv
       cases p₁ <;> simp only
-      simp [inₛ, level_based_slicing_is_sound_inₑ hn hc hr htx₁ hl₁ hel he₁ hs]
+      simp [inₛ, level_based_slicing_is_sound_inₑ hc hr htx₁ hl₁ hel he₁ hs]
   case binaryApp hop hl₁ hl₂ =>
-    specialize ihe₁ hn hs hc hr htx₁ hl₁
-    specialize ihe₂ hn hs hc hr htx₂ hl₂
+    specialize ihe₁ hs hc hr htx₁ hl₁
+    specialize ihe₂ hs hc hr htx₂ hl₂
     rw [ihe₁, ihe₂]
     simp [(@not_dereferencing_apply₂_invariant_entities op entities slice · · hop)]
