cedar-lean/Cedar/Thm/Validation/Slice/IfThenElse.lean
@@ -35,7 +35,7 @@ theorem checked_eval_entity_reachable_ite {e₁ e₂ e₃: Expr} {n : Nat} {c c'
   (hc : CapabilitiesInvariant c request entities)
   (hr : RequestAndEntitiesMatchEnvironment env request entities)
   (ht : typeOf (.ite e₁ e₂ e₃) c env = .ok (tx, c'))
-  (hl : TypedExpr.AtLevel tx n nmax)
+  (hl : TypedExpr.EntityAccessAtLevel tx n nmax)
   (hel : ¬ TypedExpr.EntityLitViaPath tx path)
   (he : evaluate (.ite e₁ e₂ e₃) request entities = .ok v)
   (ha : Value.EuidViaPath v path euid)
